compcert/common/Memory.v
@@ -26,6 +26,7 @@
 - [free]: invalidate a memory block.
 *)
 
+Require Import Zwf.
 Require Import Axioms.
 Require Import Coqlib.
 Require Import Maps.
@@ -35,6 +36,10 @@ Require Import Floats.
 Require Import Values.
 Require Export Memdata.
 Require Export Memtype.
+
+(* To avoid useless definitions of inductors in extracted code. *)
+Local Unset Elimination Schemes.
+Local Unset Case Analysis Schemes.
 
 Local Notation "a # b" := (ZMap.get b a) (at level 1).
 
@@ -151,7 +156,7 @@ Remark perm_order_dec:
   forall p1 p2, {perm_order p1 p2} + {~perm_order p1 p2}.
 Proof.
   intros. destruct p1; destruct p2; (left; constructor) || (right; intro PO; inversion PO).
-Qed.
+Defined.
 
 Remark perm_order'_dec:
   forall op p, {perm_order' op p} + {~perm_order' op p}.
@@ -159,14 +164,14 @@ Proof.
   intros. destruct op; unfold perm_order'.
   apply perm_order_dec.
   right; tauto.
-Qed.
+Defined.
 
 Theorem perm_dec:
   forall m b ofs k p, {perm m b ofs k p} + {~ perm m b ofs k p}.
 Proof.
   unfold perm; intros.
   apply perm_order'_dec.
-Qed.
+Defined.
 
 Definition range_perm (m: mem) (b: block) (lo hi: Z) (k: perm_kind) (p: permission) : Prop :=
   forall ofs, lo <= ofs < hi -> perm m b ofs k p.
@@ -198,19 +203,15 @@ Lemma range_perm_dec:
   forall m b lo hi k p, {range_perm m b lo hi k p} + {~ range_perm m b lo hi k p}.
 Proof.
   intros. 
-  assert (forall n, 0 <= n ->
-          {range_perm m b lo (lo + n) k p} + {~ range_perm m b lo (lo + n) k p}).
-    apply natlike_rec2.
-    left. red; intros. omegaContradiction.
-    intros. destruct H0. 
-    destruct (perm_dec m b (lo + z) k p). 
-    left. red; intros. destruct (zeq ofs (lo + z)). congruence. apply r. omega. 
-    right; red; intro. elim n. apply H0. omega. 
-    right; red; intro. elim n. red; intros. apply H0. omega. 
+  induction lo using (well_founded_induction_type (Zwf_up_well_founded hi)).
   destruct (zlt lo hi).
-  replace hi with (lo + (hi - lo)) by omega. apply H. omega.
-  left; red; intros. omegaContradiction. 
-Qed.
+  destruct (perm_dec m b lo k p).
+  destruct (H (lo + 1)). red. omega. 
+  left; red; intros. destruct (zeq lo ofs). congruence. apply r. omega. 
+  right; red; intros. elim n. red; intros; apply H0; omega.
+  right; red; intros. elim n. apply H0. omega. 
+  left; red; intros. omegaContradiction.
+Defined.
 
 (** [valid_access m chunk b ofs p] holds if a memory access
     of the given chunk is possible in [m] at address [b, ofs]
@@ -285,11 +286,10 @@ Proof.
   left; constructor; auto.
   right; red; intro V; inv V; contradiction.
   right; red; intro V; inv V; contradiction.
-Qed.
+Defined.
 
-(** [valid_pointer] is a boolean-valued function that says whether
-    the byte at the given location is nonempty. *)
-
+(** [valid_pointer m b ofs] returns [true] if the address [b, ofs]
+  is nonempty in [m] and [false] if it is empty. *)
 Definition valid_pointer (m: mem) (b: block) (ofs: Z): bool :=
   perm_dec m b ofs Cur Nonempty.
 
@@ -311,6 +311,28 @@ Proof.
   split. simpl; red; intros. replace ofs0 with ofs by omega. auto.
   simpl. apply Zone_divide. 
   destruct H. apply H. simpl. omega.
+Qed.
+
+(** C allows pointers one past the last element of an array.  These are not
+  valid according to the previously defined [valid_pointer]. The property
+  [weak_valid_pointer m b ofs] holds if address [b, ofs] is a valid pointer
+  in [m], or a pointer one past a valid block in [m].  *)
+
+Definition weak_valid_pointer (m: mem) (b: block) (ofs: Z) :=
+  valid_pointer m b ofs || valid_pointer m b (ofs - 1).
+
+Lemma weak_valid_pointer_spec:
+  forall m b ofs,
+  weak_valid_pointer m b ofs = true <->
+    valid_pointer m b ofs = true \/ valid_pointer m b (ofs - 1) = true.
+Proof.
+  intros. unfold weak_valid_pointer. now rewrite orb_true_iff.
+Qed.
+Lemma valid_pointer_implies:
+  forall m b ofs,
+  valid_pointer m b ofs = true -> weak_valid_pointer m b ofs = true.
+Proof.
+  intros. apply weak_valid_pointer_spec. auto.
 Qed.
 
 (** * Operations over memory stores *)
@@ -852,7 +874,7 @@ Proof.
   destruct (valid_access_dec m1 chunk b ofs Writable).
   eauto.
   contradiction.
-Qed.
+Defined.
 
 Hint Local Resolve valid_access_store: mem.
 
@@ -1338,7 +1360,7 @@ Proof.
   destruct (range_perm_dec m1 b ofs (ofs + Z_of_nat (length bytes)) Cur Writable).
   reflexivity. 
   contradiction.
-Qed.
+Defined.
 
 Theorem storebytes_store:
   forall m1 b ofs chunk v m2,
@@ -1749,7 +1771,7 @@ Theorem range_perm_free:
   { m2: mem | free m1 b lo hi = Some m2 }.
 Proof.
   intros; unfold free. rewrite pred_dec_true; auto. econstructor; eauto.
-Qed.
+Defined.
 
 Section FREE.
 
@@ -1924,7 +1946,7 @@ Theorem range_perm_drop_2:
 Proof.
   unfold drop_perm; intros. 
   destruct (range_perm_dec m b lo hi Cur Freeable). econstructor. eauto. contradiction.
-Qed.
+Defined.
 
 Section DROP.
 
@@ -2887,6 +2909,15 @@ Proof.
   eapply valid_access_extends; eauto.
 Qed.
 
+Theorem weak_valid_pointer_extends:
+  forall m1 m2 b ofs,
+  extends m1 m2 ->
+  weak_valid_pointer m1 b ofs = true -> weak_valid_pointer m2 b ofs = true.
+Proof.
+  intros until 1. unfold weak_valid_pointer. rewrite !orb_true_iff.
+  intros []; eauto using valid_pointer_extends.
+Qed.
+
 (** * Memory injections *)
 
 (** A memory state [m1] injects into another memory state [m2] via the
@@ -2899,7 +2930,8 @@ Qed.
 - if [f b = Some(b', delta)], [b'] must be valid in [m2];
 - distinct blocks in [m1] are mapped to non-overlapping sub-blocks in [m2];
 - the sizes of [m2]'s blocks are representable with unsigned machine integers;
-- the offsets [delta] are representable with unsigned machine integers.
+- pointers that could be represented using unsigned machine integers remain
+  representable after the injection.
 *)
 
 Record inject' (f: meminj) (m1 m2: mem) : Prop :=
@@ -2913,12 +2945,11 @@ Record inject' (f: meminj) (m1 m2: mem) : Prop :=
     mi_no_overlap:
       meminj_no_overlap f m1;
     mi_representable:
-      forall b b' delta ofs k p,
+      forall b b' delta ofs,
       f b = Some(b', delta) ->
-      perm m1 b (Int.unsigned ofs) k p ->
+      weak_valid_pointer m1 b (Int.unsigned ofs) = true ->
       delta >= 0 /\ 0 <= Int.unsigned ofs + delta <= Int.max_unsigned
   }.
-
 Definition inject := inject'.
 
 Local Hint Resolve mi_mappedblocks: mem.
@@ -2987,6 +3018,18 @@ Proof.
   eapply valid_access_inject; eauto.
 Qed.
 
+Theorem weak_valid_pointer_inject:
+  forall f m1 m2 b1 ofs b2 delta,
+  f b1 = Some(b2, delta) ->
+  inject f m1 m2 ->
+  weak_valid_pointer m1 b1 ofs = true ->
+  weak_valid_pointer m2 b2 (ofs + delta) = true.
+Proof.
+  intros until 2. unfold weak_valid_pointer. rewrite !orb_true_iff.
+  replace (ofs + delta - 1) with ((ofs - 1) + delta) by omega.
+  intros []; eauto using valid_pointer_inject.
+Qed.
+
 (** The following lemmas establish the absence of machine integer overflow
   during address computations. *)
 
@@ -3006,17 +3049,19 @@ Qed.
 *)
 
 Lemma address_inject:
-  forall f m1 m2 b1 ofs1 b2 delta,
+  forall f m1 m2 b1 ofs1 b2 delta p,
   inject f m1 m2 ->
-  perm m1 b1 (Int.unsigned ofs1) Max Nonempty ->
+  perm m1 b1 (Int.unsigned ofs1) Cur p ->
   f b1 = Some (b2, delta) ->
   Int.unsigned (Int.add ofs1 (Int.repr delta)) = Int.unsigned ofs1 + delta.
 Proof.
-  intros.
+  intros. apply (perm_implies _ _ _ _ _ Nonempty) in H0; [| constructor].
+  rewrite <-valid_pointer_nonempty_perm in H0.
+  apply valid_pointer_implies in H0.
   exploit mi_representable; eauto. intros [A B].
   assert (0 <= delta <= Int.max_unsigned).
     generalize (Int.unsigned_range ofs1). omega.
-  unfold Int.add. repeat rewrite Int.unsigned_repr; auto.
+  unfold Int.add. repeat rewrite Int.unsigned_repr; omega.
 Qed.
 
 Lemma address_inject':
@@ -3027,22 +3072,29 @@ Lemma address_inject':
   Int.unsigned (Int.add ofs1 (Int.repr delta)) = Int.unsigned ofs1 + delta.
 Proof.
   intros. destruct H0. eapply address_inject; eauto. 
-  apply perm_cur_max. apply H0. generalize (size_chunk_pos chunk). omega. 
+  apply H0. generalize (size_chunk_pos chunk). omega. 
+Qed.
+
+Theorem weak_valid_pointer_inject_no_overflow:
+  forall f m1 m2 b ofs b' delta,
+  inject f m1 m2 ->
+  weak_valid_pointer m1 b (Int.unsigned ofs) = true ->
+  f b = Some(b', delta) ->
+  0 <= Int.unsigned ofs + Int.unsigned (Int.repr delta) <= Int.max_unsigned.
+Proof.
+  intros. exploit mi_representable; eauto. intros.
+  pose proof (Int.unsigned_range ofs).
+  rewrite Int.unsigned_repr; omega.
 Qed.
 
 Theorem valid_pointer_inject_no_overflow:
-  forall f m1 m2 b ofs b' x,
+  forall f m1 m2 b ofs b' delta,
   inject f m1 m2 ->
   valid_pointer m1 b (Int.unsigned ofs) = true ->
-  f b = Some(b', x) ->
-  0 <= Int.unsigned ofs + Int.unsigned (Int.repr x) <= Int.max_unsigned.
+  f b = Some(b', delta) ->
+  0 <= Int.unsigned ofs + Int.unsigned (Int.repr delta) <= Int.max_unsigned.
 Proof.
-  intros. rewrite valid_pointer_valid_access in H0.
-  assert (perm m1 b (Int.unsigned ofs) Cur Nonempty).
-    apply H0. simpl. omega.
-  exploit mi_representable; eauto. intros [A B].
-  rewrite Int.unsigned_repr; auto.
-  generalize (Int.unsigned_range ofs). omega.
+  eauto using weak_valid_pointer_inject_no_overflow, valid_pointer_implies.
 Qed.
 
 Theorem valid_pointer_inject_val:
@@ -3056,6 +3108,19 @@ Proof.
   erewrite address_inject'; eauto. 
   eapply valid_pointer_inject; eauto.
   rewrite valid_pointer_valid_access in H0. eauto.
+Qed.
+
+Theorem weak_valid_pointer_inject_val:
+  forall f m1 m2 b ofs b' ofs',
+  inject f m1 m2 ->
+  weak_valid_pointer m1 b (Int.unsigned ofs) = true ->
+  val_inject f (Vptr b ofs) (Vptr b' ofs') ->
+  weak_valid_pointer m2 b' (Int.unsigned ofs') = true.
+Proof.
+  intros. inv H1. exploit mi_representable; try eassumption. intros.
+  pose proof (Int.unsigned_range ofs).
+  exploit weak_valid_pointer_inject; eauto.
+  unfold Int.add. repeat rewrite Int.unsigned_repr; auto; omega.
 Qed.
 
 Theorem inject_no_overlap:
@@ -3213,7 +3278,10 @@ Proof.
 (* no overlap *)
   red; intros. eauto with mem.
 (* representable *)
-  eauto with mem. 
+  intros. eapply mi_representable; try eassumption.
+  rewrite weak_valid_pointer_spec in *.
+  rewrite !valid_pointer_nonempty_perm in H4 |- *.
+  destruct H4; eauto with mem.
 Qed.
 
 Theorem store_unmapped_inject:
@@ -3234,7 +3302,10 @@ Proof.
 (* no overlap *)
   red; intros. eauto with mem.
 (* representable *)
-  eauto with mem.
+  intros. eapply mi_representable; try eassumption.
+  rewrite weak_valid_pointer_spec in *.
+  rewrite !valid_pointer_nonempty_perm in H3 |- *.
+  destruct H3; eauto with mem.
 Qed.
 
 Theorem store_outside_inject:
@@ -3299,7 +3370,10 @@ Proof.
 (* no overlap *)
   red; intros. eapply mi_no_overlap0; eauto; eapply perm_storebytes_2; eauto. 
 (* representable *)
-  intros. eapply mi_representable0; eauto. eapply perm_storebytes_2; eauto. 
+  intros. eapply mi_representable0; eauto.
+  rewrite weak_valid_pointer_spec in *.
+  rewrite !valid_pointer_nonempty_perm in H4 |- *.
+  destruct H4; eauto using perm_storebytes_2. 
 Qed.
 
 Theorem storebytes_unmapped_inject:
@@ -3320,7 +3394,10 @@ Proof.
 (* no overlap *)
   red; intros. eapply mi_no_overlap0; eauto; eapply perm_storebytes_2; eauto. 
 (* representable *)
-  intros. eapply mi_representable0; eauto. eapply perm_storebytes_2; eauto. 
+  intros. eapply mi_representable0; eauto.
+  rewrite weak_valid_pointer_spec in *.
+  rewrite !valid_pointer_nonempty_perm in H3 |- *.
+  destruct H3; eauto using perm_storebytes_2.
 Qed.
 
 Theorem storebytes_outside_inject:
@@ -3406,8 +3483,11 @@ Proof.
   exploit perm_alloc_inv. eauto. eexact H7. rewrite zeq_false; auto. 
 (* representable *)
   unfold f'; intros.
-  exploit perm_alloc_inv; eauto. 
-  destruct (zeq b b1). congruence. eauto with mem.
+  destruct (zeq b b1); try discriminate.
+  eapply mi_representable0; try eassumption.
+  rewrite weak_valid_pointer_spec in *.
+  rewrite !valid_pointer_nonempty_perm in H4 |- *.
+  destruct H4; eauto using perm_alloc_4.
 (* incr *)
   split. auto. 
 (* image *)
@@ -3422,7 +3502,7 @@ Theorem alloc_left_mapped_inject:
   alloc m1 lo hi = (m1', b1) ->
   valid_block m2 b2 ->
   0 <= delta <= Int.max_unsigned ->
-  (forall ofs k p, perm m2 b2 ofs k p -> delta = 0 \/ 0 <= ofs <= Int.max_unsigned) ->
+  (forall ofs k p, perm m2 b2 ofs k p -> delta = 0 \/ 0 <= ofs < Int.max_unsigned) ->
   (forall ofs k p, lo <= ofs < hi -> perm m2 b2 (ofs + delta) k p) ->
   inj_offset_aligned delta (hi-lo) ->
   (forall b delta' ofs k p,
@@ -3478,11 +3558,20 @@ Proof.
     eapply H6; eauto. omega.
   eauto.
 (* representable *)
-  unfold f'; intros. exploit perm_alloc_inv; eauto. destruct (zeq b b1); intros.
-  inversion H9; subst b' delta0. exploit H3. apply H4 with (k := k) (p := p); eauto.
-  intros [A | A]. generalize (Int.unsigned_range_2 ofs). omega.
-  generalize (Int.unsigned_range_2 ofs). omega.
-  eauto.
+  unfold f'; intros.
+  rewrite weak_valid_pointer_spec in *.
+  rewrite !valid_pointer_nonempty_perm in H10.
+  destruct (zeq b b1).
+   subst. injection H9; intros; subst b' delta0. destruct H10.
+    exploit perm_alloc_inv; eauto; rewrite zeq_true; intro.
+    exploit H3. apply H4 with (k := Cur) (p := Nonempty); eauto.
+    generalize (Int.unsigned_range_2 ofs). omega.
+   exploit perm_alloc_inv; eauto; rewrite zeq_true; intro.
+   exploit H3. apply H4 with (k := Cur) (p := Nonempty); eauto.
+   generalize (Int.unsigned_range_2 ofs). omega.
+  eapply mi_representable0; try eassumption.
+  rewrite !weak_valid_pointer_spec, !valid_pointer_nonempty_perm.
+  destruct H10; eauto using perm_alloc_4.
 (* incr *)
   split. auto.
 (* image of b1 *)
@@ -3537,7 +3626,10 @@ Proof.
 (* no overlap *)
   red; intros. eauto with mem. 
 (* representable *)
-  eauto with mem. 
+  intros. eapply mi_representable0; try eassumption.
+  rewrite weak_valid_pointer_spec in *.
+  rewrite !valid_pointer_nonempty_perm in H2 |- *.
+  destruct H2; eauto with mem.
 Qed.
 
 Lemma free_list_left_inject:
@@ -3686,9 +3778,13 @@ Proof.
   set (ofs' := Int.repr (Int.unsigned ofs + delta1)).
   assert (Int.unsigned ofs' = Int.unsigned ofs + delta1). 
     unfold ofs'; apply Int.unsigned_repr. auto.
-  exploit mi_representable1. eauto. instantiate (3 := ofs'). 
-  rewrite H. eapply perm_inj; eauto. rewrite H. intros [C D].
-  omega.
+  exploit mi_representable1. eauto. instantiate (1 := ofs').
+  rewrite H.
+  rewrite weak_valid_pointer_spec, !valid_pointer_nonempty_perm in *.
+  replace (Int.unsigned ofs + delta1 - 1) with
+    ((Int.unsigned ofs - 1) + delta1) by omega.
+  destruct H0; eauto using perm_inj.
+  rewrite H. omega.
 Qed.
 
 Lemma val_lessdef_inject_compose:
@@ -3721,7 +3817,9 @@ Proof.
 (* no overlap *)
   red; intros. eapply mi_no_overlap0; eauto; eapply perm_extends; eauto.
 (* representable *)
-  eapply mi_representable0; eauto. eapply perm_extends; eauto. 
+  eapply mi_representable0; eauto.
+  rewrite weak_valid_pointer_spec, !valid_pointer_nonempty_perm in *.
+  destruct H1; eauto using perm_extends.
 Qed.
 
 Lemma inject_extends_compose:
