compcert/cfrontend/Cexec.v
@@ -92,7 +92,7 @@ Fixpoint is_val_list (al: exprlist) : option (list (val * type)) :=
 Definition is_skip (s: statement) : {s = Sskip} + {s <> Sskip}.
 Proof.
   destruct s; (left; congruence) || (right; congruence).
-Qed.
+Defined.
 
 (** * Events, volatile memory accesses, and external functions. *)
 
@@ -303,7 +303,7 @@ Proof with try (right; intuition omega).
   destruct (zle (Int.unsigned ofs + sizeof ty) (Int.unsigned ofs')); auto.
   right; intuition omega.
   destruct Y... left; intuition omega. 
-Qed.
+Defined.
 
 Definition do_assign_loc (w: world) (ty: type) (m: mem) (b: block) (ofs: int) (v: val): option (world * trace * mem) :=
   match access_mode ty with
@@ -464,7 +464,7 @@ Proof with try (right; intuition omega).
     destruct (zle (odst + sz) osrc); auto.
     right; intuition omega.
   destruct Y... left; intuition omega.
-Qed.
+Defined.
 
 Definition do_ef_memcpy (sz al: Z)
        (w: world) (vargs: list val) (m: mem) : option (world * trace * val * mem) :=
@@ -478,10 +478,10 @@ Definition do_ef_memcpy (sz al: Z)
   | _ => None
   end.
 
-Definition do_ef_annot (text: ident) (targs: list typ)
+Definition do_ef_annot (text: ident) (targs: list annot_arg)
        (w: world) (vargs: list val) (m: mem) : option (world * trace * val * mem) :=
-  do args <- list_eventval_of_val vargs targs;
-  Some(w, Event_annot text args :: E0, Vundef, m).
+  do args <- list_eventval_of_val vargs (annot_args_typ targs);
+  Some(w, Event_annot text (annot_eventvals targs args) :: E0, Vundef, m).
 
 Definition do_ef_annot_val (text: ident) (targ: typ)
        (w: world) (vargs: list val) (m: mem) : option (world * trace * val * mem) :=
@@ -578,7 +578,8 @@ Proof with try congruence.
   econstructor. constructor; eauto. constructor.
 (* EF_inline_asm *)
   unfold do_ef_annot. destruct vargs; simpl... mydestr. 
-  split. constructor. constructor. 
+  split. change (Event_annot text nil) with (Event_annot text (annot_eventvals nil nil)).
+  constructor. constructor. 
   econstructor. constructor; eauto. constructor.
 Qed.
 
@@ -2179,7 +2180,6 @@ Proof with (unfold ret; auto with coqlib).
   rewrite H0...
   rewrite H0...
   rewrite pred_dec_false...
-  rewrite pred_dec_true...
   rewrite H0...
   rewrite H0...
   destruct H0; subst x...
