compcert/lib/Lattice.v
@@ -16,6 +16,10 @@ Require Import Coqlib.
 Require Import Maps.
 Require Import FSets.
 
+(* To avoid useless definitions of inductors in extracted code. *)
+Local Unset Elimination Schemes.
+Local Unset Case Analysis Schemes.
+
 (** * Signatures of semi-lattices *)
 
 (** A semi-lattice is a type [t] equipped with an equivalence relation [eq],
@@ -137,11 +141,15 @@ Lemma beq_correct: forall x y, beq x y = true -> eq x y.
 Proof.
   destruct x; destruct y; simpl; intro; try congruence.
   red; intro; simpl.
-  generalize (PTree.beq_correct L.eq L.beq L.beq_correct t0 t1 H p).
-  destruct (t0!p); destruct (t1!p); intuition. apply L.eq_refl.
+  rewrite PTree.beq_correct in H. generalize (H p).
+  destruct (t0!p); destruct (t1!p); intuition.
+  apply L.beq_correct; auto.
+  apply L.eq_refl. 
   red; intro; simpl.
-  generalize (PTree.beq_correct L.eq L.beq L.beq_correct t0 t1 H p).
-  destruct (t0!p); destruct (t1!p); intuition. apply L.eq_refl.
+  rewrite PTree.beq_correct in H. generalize (H p).
+  destruct (t0!p); destruct (t1!p); intuition.
+  apply L.beq_correct; auto.
+  apply L.eq_refl. 
 Qed.
 
 Definition ge (x y: t) : Prop :=
