veric/SeparationLogic.v
@@ -394,14 +394,16 @@ match op with Cop.Olt | Cop.Ogt | Cop.Ole | Cop.Oge =>
 | _ => True
 end. 
 
-
 Definition cmp_ptr_no_mem c v1 v2  :=
 match v1, v2 with
 Vptr b o, Vptr b1 o1 => 
   if zeq b b1 then
     Val.of_bool (Int.cmpu c o o1)
   else
-    force_val (Cop.sem_cmp_mismatch c)
+    match Val.cmp_different_blocks c with
+    | Some b => Val.of_bool b
+    | None => Vundef
+    end
 | _, _ => Vundef
 end. 
 
