veric/juicy_mem_lemmas.v
@@ -317,6 +317,9 @@ unfold nat_of_Z in H2.
 rewrite H5 in H2.
 unfold nat_of_P in H2.
 generalize (le_Pmult_nat p 1) as H6; intro.
+rewrite Pmult_nat_mult in H6.
+rewrite mult_1_r in H6.
+change (Pos.to_nat p) with (Z.to_nat (Z.pos p)) in H6.
 rewrite H2 in H6.
 omegaContradiction.
 assert (ofs' - ofs > 0).
@@ -827,7 +830,7 @@ split.
 unfold zle.
 case_eq (Z_le_gt_dec lo ofs); intros; auto.
 unfold zlt.
-case_eq (Z_lt_ge_dec ofs hi); intros; auto.
+case_eq (Z_lt_dec ofs hi); intros; auto.
 omegaContradiction.
 Qed.
 
